books/centaur/fgl/check-primitives.lisp
@@ -1,0 +1,420 @@
+; FGL - A Symbolic Simulation Framework for ACL2
+; Copyright (C) 2019 Centaur Technology
+;
+; Contact:
+;   Centaur Technology Formal Verification Group
+;   7600-C N. Capital of Texas Highway, Suite 300, Austin, TX 78731, USA.
+;   http://www.centtech.com/
+;
+; License: (An MIT/X11-style license)
+;
+;   Permission is hereby granted, free of charge, to any person obtaining a
+;   copy of this software and associated documentation files (the "Software"),
+;   to deal in the Software without restriction, including without limitation
+;   the rights to use, copy, modify, merge, publish, distribute, sublicense,
+;   and/or sell copies of the Software, and to permit persons to whom the
+;   Software is furnished to do so, subject to the following conditions:
+;
+;   The above copyright notice and this permission notice shall be included in
+;   all copies or substantial portions of the Software.
+;
+;   THE SOFTWARE IS PROVIDED "AS IS", WITHOUT WARRANTY OF ANY KIND, EXPRESS OR
+;   IMPLIED, INCLUDING BUT NOT LIMITED TO THE WARRANTIES OF MERCHANTABILITY,
+;   FITNESS FOR A PARTICULAR PURPOSE AND NONINFRINGEMENT. IN NO EVENT SHALL THE
+;   AUTHORS OR COPYRIGHT HOLDERS BE LIABLE FOR ANY CLAIM, DAMAGES OR OTHER
+;   LIABILITY, WHETHER IN AN ACTION OF CONTRACT, TORT OR OTHERWISE, ARISING
+;   FROM, OUT OF OR IN CONNECTION WITH THE SOFTWARE OR THE USE OR OTHER
+;   DEALINGS IN THE SOFTWARE.
+;
+; Original author: Sol Swords <sswords@centtech.com>
+
+(in-package "FGL")
+
+(include-book "add-primitives")
+(include-book "primitives-stub")
+(include-book "bfr-arithmetic")
+(include-book "def-fgl-rewrite")
+(include-book "checks")
+(local (include-book "primitive-lemmas"))
+(local (include-book "centaur/bitops/ihsext-basics" :dir :system))
+(local (std::add-default-post-define-hook :fix))
+
+(local (in-theory (disable w)))
+
+
+(def-formula-checks checks-formula-checks
+  (check-integerp
+   check-natp
+   check-int-endp
+   check-bitp
+   check-signed-byte-p
+   check-unsigned-byte-p
+   check-non-integerp
+   check-consp
+   check-non-consp
+   check-booleanp
+   check-non-booleanp
+   integer-length-bound
+   ifix))
+
+;; (local (defthm equal-of-len
+;;          (implies (syntaxp (quotep n))
+;;                   (equal (equal (len x) n)
+;;                          (cond ((equal n 0) (atom x))
+;;                                ((zp n) nil)
+;;                                ((consp x) (equal (len (cdr x)) (1- n)))
+;;                                (t nil))))))
+
+(local (defthm fgl-ev-context-equv-forall-extensions-trivial
+         (implies (acl2::rewriting-negative-literal
+                   `(fgl-ev-context-equiv-forall-extensions ,contexts ,obj ,term ,eval-alist))
+                  (iff (fgl-ev-context-equiv-forall-extensions contexts obj term eval-alist)
+                       (and 
+                        (equal (fgl-ev-context-fix contexts (fgl-ev term eval-alist))
+                               (fgl-ev-context-fix contexts obj))
+                        (hide (fgl-ev-context-equiv-forall-extensions contexts obj term eval-alist)))))
+         :hints (("goal" :expand ((:free (x) (hide x)))
+                  :use ((:instance fgl-ev-context-equiv-forall-extensions-necc
+                         (ext eval-alist)))
+                  :in-theory (disable fgl-ev-context-equiv-forall-extensions-necc)))))
+
+(local (in-theory (disable fgl-ev-context-equiv-forall-extensions)))
+
+;; (local (defthm fgl-object-bindings-eval-nil
+;;          (equal (fgl-object-bindings-eval-
+
+(local (defthm fgl-object-eval-when-booleanp
+         (implies (booleanp x)
+                  (equal (fgl-object-eval x env) x))
+         :hints(("Goal" :in-theory (enable fgl-object-eval fgl-object-kind g-concrete->val)))))
+
+(def-fgl-binder-meta check-integerp-binder
+  (if (and (eq (pseudo-fnsym-fix fn) 'check-integerp)
+           (eql (len args) 1))
+      (b* ((arg (car args))
+           (ans
+            (fgl-object-case arg
+              :g-concrete (integerp arg.val)
+              :g-integer t
+              :g-apply (or (and (eq arg.fn 'ifix) (eql (len arg.args) 1))
+                           (eq arg.fn 'intcdr)
+                           (eq arg.fn 'intcons))
+              :otherwise nil)))
+        (mv t 'ans (if ans '((ans . t)) '((ans . nil))) nil interp-st state))
+    (mv nil nil nil nil interp-st state))
+  :formula-check checks-formula-checks
+  :prepwork ((local (in-theory (enable check-integerp)))))
+
+(add-fgl-binder-meta check-integerp check-integerp-binder)
+
+
+
+
+(def-fgl-binder-meta check-natp-binder
+  (if (and (eq (pseudo-fnsym-fix fn) 'check-natp)
+           (eql (len args) 1))
+      (b* ((arg (car args))
+           (ans
+            (fgl-object-case arg
+              :g-concrete (natp arg.val)
+              :g-integer (eq (car (last arg.bits)) nil)
+              :otherwise nil)))
+        (mv t 'ans (if ans '((ans . t)) '((ans . nil))) nil interp-st state))
+    (mv nil nil nil nil interp-st state))
+  :formula-check checks-formula-checks
+  :prepwork ((local (in-theory (enable check-natp)))
+             (local (defthm bools->int-less-than-0
+                      (iff (< (bools->int x) 0)
+                           (car (last x)))
+                      :hints(("Goal" :in-theory (enable bools->int)))))
+             (local (defthm car-last-of-gobj-bfr-list-eval
+                      (implies (not (car (last x)))
+                               (not (car (last (gobj-bfr-list-eval x env)))))
+                      :hints(("Goal" :in-theory (enable gobj-bfr-list-eval)))))))
+
+(add-fgl-binder-meta check-natp check-natp-binder)
+
+
+(def-fgl-binder-meta check-int-endp-binder
+  (if (and (eq (pseudo-fnsym-fix fn) 'check-int-endp)
+           (eql (len args) 1))
+      (b* ((arg (car args))
+           (ans
+            (fgl-object-case arg
+              :g-concrete (or (not (integerp arg.val))
+                              (int-endp arg.val))
+              :g-integer (or (atom arg.bits)
+                             (atom (cdr arg.bits)))
+              :g-boolean t
+              :g-cons t
+              :otherwise nil)))
+        (mv t 'ans (if ans '((ans . t)) '((ans . nil))) nil interp-st state))
+    (mv nil nil nil nil interp-st state))
+  :formula-check checks-formula-checks
+  :prepwork ((local (in-theory (enable check-int-endp)))
+             (local (defthm int-endp-of-bools->int
+                      (implies (atom (cdr x))
+                               (int-endp (bools->int x)))
+                      :hints(("Goal" :in-theory (enable bools->int int-endp)))))
+             (local (defthm consp-cdr-of-gobj-bfr-list-eval
+                      (iff (consp (cdr (gobj-bfr-list-eval x env)))
+                           (consp (cdr x)))
+                      :hints(("Goal" :in-theory (enable gobj-bfr-list-eval)))))
+             (local (defthm int-endp-when-not-integerp
+                      (implies (not (integerp x))
+                               (int-endp x))
+                      :hints(("Goal" :in-theory (enable int-endp)))))))
+
+(add-fgl-binder-meta check-int-endp check-int-endp-binder)
+
+
+(def-fgl-binder-meta check-bitp-binder
+  (if (and (eq (pseudo-fnsym-fix fn) 'check-bitp)
+           (eql (len args) 1))
+      (b* ((arg (car args))
+           (ans
+            (fgl-object-case arg
+              :g-concrete (bitp arg.val)
+              :g-integer (or (endp arg.bits)
+                             (and (endp (cdr arg.bits))
+                                  (not (car arg.bits)))
+                             (and (consp (cdr arg.bits))
+                                  (endp (cddr arg.bits))
+                                  (not (cadr arg.bits))))
+              :otherwise nil)))
+        (mv t 'ans (if ans '((ans . t)) '((ans . nil))) nil interp-st state))
+    (mv nil nil nil nil interp-st state))
+  :formula-check checks-formula-checks
+  :prepwork ((local (in-theory (enable check-bitp)))
+             (local (defthm bitp-of-bools->int
+                      (implies (or (atom x)
+                                   (and (atom (cdr x))
+                                        (not (car x)))
+                                   (and (consp (cdr x))
+                                        (atom (cddr x))
+                                        (not (cadr x))))
+                               (bitp (bools->int x)))
+                      :hints(("Goal" :in-theory (enable bools->int bitp)))))
+             (local (defthm consp-cdr-of-gobj-bfr-list-eval
+                      (iff (consp (cdr (gobj-bfr-list-eval x env)))
+                           (consp (cdr x)))
+                      :hints(("Goal" :in-theory (enable gobj-bfr-list-eval)))))
+             (local (defthm consp-cddr-of-gobj-bfr-list-eval
+                      (iff (consp (cddr (gobj-bfr-list-eval x env)))
+                           (consp (cddr x)))
+                      :hints(("Goal" :in-theory (enable gobj-bfr-list-eval)))))
+             (local (defthm not-cadr-of-gobj-bfr-list-eval
+                      (implies (not (cadr x))
+                               (not (cadr (gobj-bfr-list-eval x env))))
+                      :hints(("Goal" :in-theory (enable gobj-bfr-list-eval)))))))
+
+(add-fgl-binder-meta check-bitp check-bitp-binder)
+
+
+
+(def-fgl-binder-meta check-signed-byte-p-binder
+  (if (and (eq (pseudo-fnsym-fix fn) 'check-signed-byte-p)
+           (eql (len args) 2))
+      (b* ((len (car args))
+           (arg (cadr args))
+           ((unless (fgl-object-case len :g-concrete))
+            (mv nil nil nil nil interp-st state))
+           (len (g-concrete->val len))
+           ((unless (posp len))
+            (mv t 'ans '((ans . nil)) nil interp-st state))
+           (ans
+            (fgl-object-case arg
+              :g-concrete (signed-byte-p len arg.val)
+              :g-integer (<= (len arg.bits) len)
+              :otherwise nil)))
+        (mv t 'ans (if ans '((ans . t)) '((ans . nil))) nil interp-st state))
+    (mv nil nil nil nil interp-st state))
+  :formula-check checks-formula-checks
+  :prepwork ((local (in-theory (enable check-signed-byte-p)))
+             (local (defun signed-byte-p-of-bools->int-ind (n x)
+                      (if (or (zp n) (eql n 1))
+                          x
+                        (signed-byte-p-of-bools->int-ind (1- n) (cdr x)))))
+
+             (local (defthm signed-byte-p-of-bools->int
+                      (implies (and (posp n)
+                                    (<= (len x) n))
+                               (signed-byte-p n (bools->int x)))
+                      :hints(("Goal" :in-theory (e/d (bools->int len bool->bit)
+                                                     (signed-byte-p
+                                                      bitops::signed-byte-p-of-logcdr))
+                              :induct (signed-byte-p-of-bools->int-ind n x)
+                              :expand ((:with bitops::signed-byte-p** (:free (x) (signed-byte-p n x))))))))
+             (local (defthm len-of-gobj-bfr-list-eval
+                      (equal (len (gobj-bfr-list-eval x env))
+                             (len x))))))
+
+(add-fgl-binder-meta check-signed-byte-p check-signed-byte-p-binder)
+
+
+(def-fgl-binder-meta check-unsigned-byte-p-binder
+  (if (and (eq (pseudo-fnsym-fix fn) 'check-unsigned-byte-p)
+           (eql (len args) 2))
+      (b* ((len (car args))
+           (arg (cadr args))
+           ((unless (fgl-object-case len :g-concrete))
+            (mv nil nil nil nil interp-st state))
+           (len (g-concrete->val len))
+           ((unless (natp len))
+            (mv t 'ans '((ans . nil)) nil interp-st state))
+           (ans
+            (fgl-object-case arg
+              :g-concrete (unsigned-byte-p len arg.val)
+              :g-integer (and (<= (len arg.bits) (+ 1 len))
+                              (not (car (last arg.bits))))
+              :otherwise nil)))
+        (mv t 'ans (if ans '((ans . t)) '((ans . nil))) nil interp-st state))
+    (mv nil nil nil nil interp-st state))
+  :formula-check checks-formula-checks
+  :prepwork ((local (in-theory (e/d (check-unsigned-byte-p)
+                                    (unsigned-byte-p))))
+             (local (defun unsigned-byte-p-of-bools->int-ind (n x)
+                      (if (zp n)
+                          x
+                        (unsigned-byte-p-of-bools->int-ind (1- n) (cdr x)))))
+
+             (local (defthm unsigned-byte-p-of-bools->int
+                      (implies (and (natp n)
+                                    (<= (len x) (+ 1 n))
+                                    (not (car (last x))))
+                               (unsigned-byte-p n (bools->int x)))
+                      :hints(("Goal" :in-theory (e/d (bools->int len last bool->bit)
+                                                     (unsigned-byte-p))
+                              :induct (unsigned-byte-p-of-bools->int-ind n x)
+                              :expand ((:with bitops::unsigned-byte-p** (:free (x) (unsigned-byte-p n x))))))))
+             (local (defthm car-last-of-gobj-bfr-list-eval
+                      (implies (not (car (last x)))
+                               (not (car (last (gobj-bfr-list-eval x env)))))
+                      :hints(("Goal" :in-theory (enable gobj-bfr-list-eval)))))))
+
+(add-fgl-binder-meta check-unsigned-byte-p check-unsigned-byte-p-binder)
+
+
+(def-fgl-binder-meta check-non-integerp-binder
+  (if (and (eq (pseudo-fnsym-fix fn) 'check-non-integerp)
+           (eql (len args) 1))
+      (b* ((arg (car args))
+           (ans
+            (fgl-object-case arg
+              :g-concrete (not (integerp arg.val))
+              :g-integer nil
+              :g-boolean t
+              :g-cons t
+              :otherwise nil)))
+        (mv t 'ans (if ans '((ans . t)) '((ans . nil))) nil interp-st state))
+    (mv nil nil nil nil interp-st state))
+  :formula-check checks-formula-checks
+  :prepwork ((local (in-theory (enable check-non-integerp)))))
+
+(add-fgl-binder-meta check-non-integerp check-non-integerp-binder)
+
+
+(def-fgl-binder-meta check-consp-binder
+  (if (and (eq (pseudo-fnsym-fix fn) 'check-consp)
+           (eql (len args) 1))
+      (b* ((arg (car args))
+           (ans
+            (fgl-object-case arg
+              :g-concrete (consp arg.val)
+              :g-integer nil
+              :g-boolean nil
+              :g-cons t
+              :g-apply (eq arg.fn 'cons)
+              :otherwise nil)))
+        (mv t 'ans (if ans '((ans . t)) '((ans . nil))) nil interp-st state))
+    (mv nil nil nil nil interp-st state))
+  :formula-check checks-formula-checks
+  :prepwork ((local (in-theory (enable check-consp)))))
+
+(add-fgl-binder-meta check-consp check-consp-binder)
+
+(def-fgl-binder-meta check-non-consp-binder
+  (if (and (eq (pseudo-fnsym-fix fn) 'check-non-consp)
+           (eql (len args) 1))
+      (b* ((arg (car args))
+           (ans
+            (fgl-object-case arg
+              :g-concrete (not (consp arg.val))
+              :g-integer t
+              :g-boolean t
+              :otherwise nil)))
+        (mv t 'ans (if ans '((ans . t)) '((ans . nil))) nil interp-st state))
+    (mv nil nil nil nil interp-st state))
+  :formula-check checks-formula-checks
+  :prepwork ((local (in-theory (enable check-non-consp)))))
+
+(add-fgl-binder-meta check-non-consp check-non-consp-binder)
+
+
+(def-fgl-binder-meta check-booleanp-binder
+  (if (and (eq (pseudo-fnsym-fix fn) 'check-booleanp)
+           (eql (len args) 1))
+      (b* ((arg (car args))
+           (ans
+            (fgl-object-case arg
+              :g-concrete (booleanp arg.val)
+              :g-boolean t
+              :g-apply (or (eq arg.fn 'equal)
+                           (eq arg.fn 'intcar)
+                           (eq arg.fn 'integerp))
+              :otherwise nil)))
+        (mv t 'ans (if ans '((ans . t)) '((ans . nil))) nil interp-st state))
+    (mv nil nil nil nil interp-st state))
+  :formula-check checks-formula-checks
+  :prepwork ((local (in-theory (enable check-booleanp)))))
+
+(add-fgl-binder-meta check-booleanp check-booleanp-binder)
+
+(def-fgl-binder-meta check-non-booleanp-binder
+  (if (and (eq (pseudo-fnsym-fix fn) 'check-non-booleanp)
+           (eql (len args) 1))
+      (b* ((arg (car args))
+           (ans
+            (fgl-object-case arg
+              :g-concrete (not (booleanp arg.val))
+              :g-integer t
+              :g-cons t
+              :otherwise nil)))
+        (mv t 'ans (if ans '((ans . t)) '((ans . nil))) nil interp-st state))
+    (mv nil nil nil nil interp-st state))
+  :formula-check checks-formula-checks
+  :prepwork ((local (in-theory (enable check-non-booleanp)))))
+
+(add-fgl-binder-meta check-non-booleanp check-non-booleanp-binder)
+
+(local (in-theory (enable fgl-object-p-when-integerp)))
+
+(def-fgl-binder-meta integer-length-bound-binder
+  (if (and (eq (pseudo-fnsym-fix fn) 'integer-length-bound)
+           (eql (len args) 1))
+      (b* ((arg (car args))
+           (ans
+            (fgl-object-case arg
+              :g-concrete (integer-length (ifix arg.val))
+              :g-boolean 0
+              :g-cons 0
+              :g-integer (max 0 (1- (len arg.bits)))
+              :otherwise nil)))
+        (mv t 'ans `((ans . ,ans)) nil interp-st state))
+    (mv nil nil nil nil interp-st state))
+  :formula-check checks-formula-checks
+  :prepwork ((local (in-theory (enable integer-length-bound
+                                       fgl-object-p-when-integerp
+                                       fgl-object-kind-when-integerp
+                                       g-concrete->val-when-integerp)))
+             (local (defthm integer-length-when-zip
+                      (implies (zip x)
+                               (equal (integer-length x) 0))))
+             (local (defthm integer-length-of-bools->int
+                      (<= (integer-length (bools->int x)) (max 0 (+ -1 (len x))))
+                      :hints(("Goal" :in-theory (enable bools->int
+                                                        bool->bit
+                                                        bitops::integer-length**)))
+                      :rule-classes ((:linear :trigger-terms ((integer-length (bools->int x)))))))))
+
+(add-fgl-binder-meta integer-length-bound integer-length-bound-binder)
