books/centaur/fgl/checks.lisp
@@ -1,0 +1,204 @@
+; FGL - A Symbolic Simulation Framework for ACL2
+; Copyright (C) 2018 Centaur Technology
+;
+; Contact:
+;   Centaur Technology Formal Verification Group
+;   7600-C N. Capital of Texas Highway, Suite 300, Austin, TX 78731, USA.
+;   http://www.centtech.com/
+;
+; License: (An MIT/X11-style license)
+;
+;   Permission is hereby granted, free of charge, to any person obtaining a
+;   copy of this software and associated documentation files (the "Software"),
+;   to deal in the Software without restriction, including without limitation
+;   the rights to use, copy, modify, merge, publish, distribute, sublicense,
+;   and/or sell copies of the Software, and to permit persons to whom the
+;   Software is furnished to do so, subject to the following conditions:
+;
+;   The above copyright notice and this permission notice shall be included in
+;   all copies or substantial portions of the Software.
+;
+;   THE SOFTWARE IS PROVIDED "AS IS", WITHOUT WARRANTY OF ANY KIND, EXPRESS OR
+;   IMPLIED, INCLUDING BUT NOT LIMITED TO THE WARRANTIES OF MERCHANTABILITY,
+;   FITNESS FOR A PARTICULAR PURPOSE AND NONINFRINGEMENT. IN NO EVENT SHALL THE
+;   AUTHORS OR COPYRIGHT HOLDERS BE LIABLE FOR ANY CLAIM, DAMAGES OR OTHER
+;   LIABILITY, WHETHER IN AN ACTION OF CONTRACT, TORT OR OTHERWISE, ARISING
+;   FROM, OUT OF OR IN CONNECTION WITH THE SOFTWARE OR THE USE OR OTHER
+;   DEALINGS IN THE SOFTWARE.
+;
+; Original author: Sol Swords <sswords@centtech.com>
+
+(in-package "FGL")
+
+(include-book "arith-base")
+(include-book "syntax-bind")
+
+(define check-integerp (ans x)
+  (and (integerp x) ans t)
+  ///
+  (defthm check-integerp-implies-integerp
+    (implies (check-integerp ans x)
+             (integerp x))
+    :rule-classes :forward-chaining)
+
+  (defmacro check-integerp! (&rest args)
+    `(binder (check-integerp . ,args))))
+
+(define check-natp (ans x)
+  (and (natp x) ans t)
+  ///
+  (defthm check-natp-implies-natp
+    (implies (check-natp ans x)
+             (natp x))
+    :rule-classes :forward-chaining)
+
+  (defmacro check-natp! (&rest args)
+    `(binder (check-natp . ,args))))
+
+(define check-int-endp (ans (x integerp))
+  (and (int-endp x) ans t)
+  ///
+  (defthm check-int-endp-fn-implies-int-endp
+    (implies (acl2::rewriting-negative-literal `(check-int-endp ,ans ,x))
+             (iff (check-int-endp ans x)
+                  (and (int-endp x)
+                       (hide (check-int-endp ans x)))))
+    :hints(("Goal" :expand ((:free (x) (hide x))))))
+
+  (defmacro check-int-endp! (&rest args)
+    `(binder (check-int-endp . ,args))))
+
+(define check-bitp (ans x)
+  (and (bitp x) ans t)
+  ///
+  (defthm check-bitp-implies-bitp
+    (implies (check-bitp ans x)
+             (bitp x))
+    :rule-classes :forward-chaining)
+
+  (defmacro check-bitp! (&rest args)
+    `(binder (check-bitp . ,args))))
+
+(define check-signed-byte-p (ans n x)
+  (and (signed-byte-p n x) ans t)
+  ///
+  (defthm check-signed-byte-p-implies-signed-byte-p
+    (implies (acl2::rewriting-negative-literal `(check-signed-byte-p ,ans ,n ,x))
+             (iff (check-signed-byte-p ans n x)
+                  (and (signed-byte-p n x)
+                       (hide (check-signed-byte-p ans n x)))))
+    :hints(("Goal" :expand ((:free (x) (hide x))))))
+
+  (defmacro check-signed-byte-p! (&rest args)
+    `(binder (check-signed-byte-p . ,args))))
+
+(define check-unsigned-byte-p (ans n x)
+  (and (unsigned-byte-p n x) ans t)
+  ///
+  (defthm check-unsigned-byte-p-implies-unsigned-byte-p
+    (implies (acl2::rewriting-negative-literal `(check-unsigned-byte-p ,ans ,n ,x))
+             (iff (check-unsigned-byte-p ans n x)
+                  (and (unsigned-byte-p n x)
+                       (hide (check-unsigned-byte-p ans n x)))))
+    :hints(("Goal" :expand ((:free (x) (hide x))))))
+
+  (defmacro check-unsigned-byte-p! (&rest args)
+    `(binder (check-unsigned-byte-p . ,args))))
+
+
+(define check-non-integerp (ans x)
+  (and (not (integerp x))
+       ans
+       t)
+  ///
+  (defthm check-non-integerp-implies-not-integerp
+    (implies (check-non-integerp ans x)
+             (not (integerp x)))
+    :rule-classes :forward-chaining)
+
+  (defmacro check-non-integerp! (&rest args)
+    `(binder (check-non-integerp . ,args))))
+
+(define check-consp (ans x)
+  (and (consp x)
+       ans
+       t)
+  ///
+  (defthm check-consp-implies-consp
+    (implies (check-consp ans x)
+             (consp x))
+    :rule-classes :forward-chaining)
+
+  (defmacro check-consp! (&rest args)
+    `(binder (check-consp . ,args))))
+
+(define check-non-consp (ans x)
+  (and (not (consp x))
+       ans
+       t)
+  ///
+  (defthm check-non-consp-implies-not-consp
+    (implies (check-non-consp ans x)
+             (not (consp x)))
+    :rule-classes :forward-chaining)
+
+  (defmacro check-non-consp! (&rest args)
+    `(binder (check-non-consp . ,args))))
+
+(define check-booleanp (ans x)
+  (and (booleanp x)
+       ans
+       t)
+  ///
+  (defthm check-booleanp-implies-booleanp
+    (implies (check-booleanp ans x)
+             (booleanp x))
+    :rule-classes :forward-chaining)
+
+  (defmacro check-booleanp! (&rest args)
+    `(binder (check-booleanp . ,args))))
+
+(define check-non-booleanp (ans x)
+  (and (not (booleanp x))
+       ans
+       t)
+  ///
+  (defthm check-non-booleanp-implies-not-booleanp
+    (implies (check-non-booleanp ans x)
+             (not (booleanp x)))
+    :rule-classes :forward-chaining)
+
+  (defmacro check-non-booleanp! (&rest args)
+    `(binder (check-non-booleanp . ,args))))
+
+
+
+(define integer-length-bound ((ans acl2::maybe-natp) (x integerp))
+  :returns (bound acl2::maybe-natp :rule-classes :type-prescription)
+  (and (natp ans)
+       (<= (integer-length x) ans)
+       ans)
+  ///
+  (defthm integer-length-bound-implies-integer-length
+    (implies (integer-length-bound ans x)
+             (<= (integer-length x) (integer-length-bound ans x)))
+    :hints (("goal" :expand ((:free (x) (hide x)))))
+    :rule-classes :linear)
+
+  (defmacro integer-length-bound! (&rest args)
+    `(binder (integer-length-bound . ,args))))
+
+
+
+(define check-equal (ans x y)
+  (and (equal x y)
+       ans
+       t)
+  ///
+  (defthm check-equal-implies-equal
+    (implies (check-equal ans x y)
+             (equal x y))
+    :rule-classes :forward-chaining)
+
+  (defmacro check-equal! (&rest args)
+    `(binder (check-equal . ,args))))
