books/centaur/fgl/trace.lisp
@@ -31,50 +31,54 @@
 (in-package "FGL")
 
 (include-book "interp-st")
-(include-book "rules")
+(include-book "binder-rules")
 
 
 
 (encapsulate
-  (((fgl-rewrite-try-rule-trace * * * interp-st state) => interp-st
-    :formals (status rule call interp-st state)
-    :guard (and (fgl-rule-p rule)
-                (fgl-object-p call))))
+  (((fgl-rewrite-try-rule-trace * * * * interp-st state) => interp-st
+    :formals (status rule fn args interp-st state)
+    :guard (and (fgl-generic-rule-p rule)
+                (pseudo-fnsym-p fn)
+                (fgl-objectlist-p args))))
 
   (set-ignore-ok t)
   (set-irrelevant-formals-ok t)
-  (local (defun fgl-rewrite-try-rule-trace (status rule call interp-st state)
+  (local (defun fgl-rewrite-try-rule-trace (status rule fn args interp-st state)
            (declare (xargs :stobjs (interp-st state)
-                           :guard (and (pseudo-rewrite-rule-p rule)
-                                       (fgl-object-p call))))
+                           :guard (and (fgl-generic-rule-p rule)
+                                       (pseudo-fnsym-p fn)
+                                       (fgl-objectlist-p args))))
            interp-st))
 
   (defthm interp-st-get-of-fgl-rewrite-try-rule-trace
     (implies (not (equal (interp-st-field-fix key) :trace-scratch))
-             (equal (interp-st-get key (fgl-rewrite-try-rule-trace status rule call interp-st state))
+             (equal (interp-st-get key (fgl-rewrite-try-rule-trace status rule fn args interp-st state))
                     (interp-st-get key interp-st)))))
 
 (define fgl-rewrite-try-rule-trace-wrapper (trace
-                                           status
-                                           (rule fgl-rule-p)
-                                           (call fgl-object-p)
-                                           interp-st
-                                           state)
+                                            status
+                                            (rule fgl-generic-rule-p)
+                                            (fn pseudo-fnsym-p)
+                                            (args fgl-objectlist-p)
+                                            interp-st
+                                            state)
   :inline t
   (if trace
-      (fgl-rewrite-try-rule-trace status rule call interp-st state)
+      (fgl-rewrite-try-rule-trace status rule fn args interp-st state)
     interp-st)
   ///
   (defthm interp-st-get-of-fgl-rewrite-try-rule-trace-wrapper
     (implies (not (equal (interp-st-field-fix key) :trace-scratch))
              (equal (interp-st-get key (fgl-rewrite-try-rule-trace-wrapper
-                                        trace status rule call interp-st state))
+                                        trace status rule fn args interp-st state))
                     (interp-st-get key interp-st)))))
 
 
 (define fgl-rewrite-rule-try-trace-default (status
-                                           (rule fgl-rule-p)
-                                           (call fgl-object-p)
+                                           (rule fgl-generic-rule-p)
+                                           (fn pseudo-fnsym-p)
+                                           (args fgl-objectlist-p)
                                            interp-st state)
   :returns new-interp-st
   (b* ((rule-alist (and (boundp-global :fgl-trace-rule-alist state)
@@ -82,7 +86,7 @@
        ((unless (alistp rule-alist))
         (er hard? 'fgl-rewrite-rule-try-trace-default "Bad :fgl-trace-rule-alist -- not an alist")
         interp-st)
-       (rune (fgl-rule->rune rule))
+       (rune (fgl-generic-rule->rune rule))
        (look (assoc-equal rune rule-alist))
        ((unless look)
         interp-st)
@@ -93,7 +97,7 @@
       (':start
        (prog2$ (fmt-to-comment-window
                 "~t0~x1> ~x2 ~x3~%"
-                (pairlis2 acl2::*base-10-chars* (list depth depth rune call))
+                (pairlis2 acl2::*base-10-chars* (list depth depth rune (g-apply fn args)))
                 0 evisc-tuple nil)
                (update-interp-st->trace-scratch (1+ depth) interp-st)))
       ((':hyps . failed-hyp)
@@ -196,7 +200,9 @@ following inputs:</p>
 <li>@('rule'), the rewrite rule structure of the rule being attempted, with
 guard @('(pseudo-rewrite-rule-p rule)')</li>
 
-<li>@('call'), the term to be rewritten, with which the LHS was unified</li>
+<li>@('fn'), the function of the call being rewritten</li>
+
+<li>@('args'), the arguments of the call being rewritten</li>
 
 <li>@('interp-st'), the FGL interpreter state</li>
 
